mlir: use MLIRTy rather than Type in SSA value storage

MLIRSemantics/SSAEnv.lean
@@ -3,7 +3,7 @@
 
 This file implements the SSA environment which maps variables names from
 different scopes to explicitly-typed values. It is, conceptually, a map
-`SSAVal → (α: Type) × α` for each scope.
+`SSAVal → (α: MLIRTy) × α` for each scope.
 
 The main concern with such state is the definition, maintainance and use of the
 property that the values are defined only once, allowing us to study sections
@@ -27,7 +27,9 @@ care when proving the correction of transformations.
 TODO:
  1. How to guarantee that read values exist and have the proper type without
     going too deep into proofs?
- 2. Document events
+    => Use default values! Data is always inhabited.
+ 2. Improve the typing: auto-simplify τ.eval and the resulting casts
+ 3. Set up infrastructure to unpack MLIRTy types into Lean native stuff
 
 Linking definitions and operations:
  1. run (%a = 2) in environment env :: whatever
@@ -46,10 +48,13 @@ Block scoping: operation o1 can branch to block b2 if:
  - b2 is in the same region as the block owning o1
 -/
 
+import MLIRSemantics.Fitree
+
 import MLIR.AST
 open MLIR.AST
 
--- Shortcuts for SSAVal
+
+-- Additional definitions for MLIR.AST types
 
 instance: Coe String SSAVal where
   coe := SSAVal.SSAVal
@@ -64,23 +69,73 @@ def SSAVal.decEq (v1 v2: SSAVal): Decidable (Eq v1 v2) :=
 instance: DecidableEq SSAVal :=
   SSAVal.decEq
 
+deriving instance DecidableEq for Dimension
+
+def MLIRTy.beq (t1 t2: MLIRTy): Bool :=
+  match t1, t2 with
+  | MLIRTy.fn a1 b1, MLIRTy.fn a2 b2 =>
+      beq a1 a2 && beq b1 b2
+  | MLIRTy.int n1, MLIRTy.int n2 =>
+      n1 == n2
+  | MLIRTy.float n1, MLIRTy.float n2 =>
+      n1 == n2
+  | MLIRTy.tuple [], MLIRTy.tuple [] =>
+      true
+  | MLIRTy.tuple (t1::l1), MLIRTy.tuple (t2::l2) =>
+      beq t1 t2 && beq (MLIRTy.tuple l1) (MLIRTy.tuple l2)
+  | MLIRTy.vector l1 t1, MLIRTy.vector l2 t2 =>
+      l1 == l2 && beq t1 t2
+  | MLIRTy.tensor l1 t1, MLIRTy.tensor l2 t2 =>
+      l1 == l2 && beq t1 t2
+  | MLIRTy.user n1, MLIRTy.user n2 =>
+      n1 == n2
+  | _, _ =>
+      false
+
+def MLIRTy.decEq (t1 t2: MLIRTy): Decidable (Eq t1 t2) :=
+  if MLIRTy.beq t1 t2 then isTrue sorry else isFalse sorry
+
+instance: DecidableEq MLIRTy :=
+  MLIRTy.decEq
+
+
+-- Evaluation of MLIR types
+-- TODO: Not all MLIRTy types are correctly evaluated
+
+@[simp, inline]
+def MLIR.AST.MLIRTy.eval: MLIRTy → Type
+  | MLIRTy.fn τ₁ τ₂ => τ₁.eval → τ₂.eval
+  | MLIRTy.int _ => Int
+  | MLIRTy.float _ => Float
+  | MLIRTy.tuple [] => Unit
+  | MLIRTy.tuple [τ] => τ.eval
+  | MLIRTy.tuple (τ::l) => τ.eval × (MLIRTy.tuple l).eval
+  | MLIRTy.vector _ _ => Unit /- todo -/
+  | MLIRTy.tensor _ _ => Unit /- todo -/
+  | MLIRTy.user _ => Unit /- todo -/
+
+
 -- SSAScope
 
 def SSAScope :=
-  List (SSAVal × (α: Type) × α)
+  List (SSAVal × (τ: MLIRTy) × τ.eval)
 
 @[simp]
-def SSAScope.get (name: SSAVal): SSAScope → Option ((α: Type) × α)
-  | [] => none
-  | ⟨name', α, v⟩ :: l => if name' = name then some ⟨α, v⟩ else get name l
+def SSAScope.get (name: SSAVal): SSAScope → (τ: MLIRTy) → Option τ.eval
+  | [], _ => none
+  | ⟨name', τ', v'⟩ :: l, τ =>
+      if H: name' = name && τ' = τ then
+        some (cast (by simp at H; simp [H]) v')
+      else get name l τ
 
 @[simp]
-def SSAScope.set {α} (name: SSAVal) (v: α): SSAScope → SSAScope
-  | [] => [⟨name, α, v⟩]
-  | ⟨name', β, v'⟩ :: l =>
+def SSAScope.set (name: SSAVal) (τ: MLIRTy) (v: τ.eval):
+      SSAScope → SSAScope
+  | [] => [⟨name, τ, v⟩]
+  | ⟨name', τ', v'⟩ :: l =>
       if name' = name
-      then ⟨name', α, v⟩ :: l
-      else ⟨name', β, v'⟩ :: set name v l
+      then ⟨name', τ, v⟩ :: l
+      else ⟨name', τ', v'⟩ :: set name τ v l
 
 /- Maybe useful in the future, for proofs
 def SSAScope.has (name: SSAVal) (l: SSAScope): Bool :=
@@ -89,8 +144,9 @@ def SSAScope.has (name: SSAVal) (l: SSAScope): Bool :=
 def SSAScope.free (name: SSAVal) (l: SSAScope): Bool :=
   l.all (fun ⟨name', _, _⟩ => name' != name)
 
-def SSAScope.maps (l: SSAScope) {α} (name: SSAVal) (value: α): Prop :=
-  l.Mem ⟨name, α, value⟩ -/
+def SSAScope.maps (l: SSAScope) (name: SSAVal) (τ: MLIRTy) (v: τ.eval) :=
+  l.Mem ⟨name, τ, v⟩ -/
+
 
 -- SSAEnv
 
@@ -98,39 +154,54 @@ def SSAEnv :=
   List SSAScope
 
 @[simp]
-def SSAEnv.get (name: SSAVal): SSAEnv → Option ((α: Type) × α)
+def SSAEnv.get (name: SSAVal) (τ: MLIRTy): SSAEnv → Option τ.eval
   | [] => none
   | l :: s =>
-      match l.get name with
-      | none => get name s
+      match l.get name τ with
+      | none => get name τ s
       | some v => v
 
 @[simp]
-def SSAEnv.set {α} (name: SSAVal) (v: α): SSAEnv → SSAEnv
+def SSAEnv.set (name: SSAVal) (τ: MLIRTy) (v: τ.eval): SSAEnv → SSAEnv
   | [] => [] -- cannot happen in practice
-  | l :: s => l.set name v :: s
+  | l :: s => l.set name τ v :: s
 
 /- Useful for proofs
 def SSAEnv.refines (new old: SSAEnv) :=
-  ∀ ⦃name v⦄, old.get name = some v → new.get name = some v
+  ∀ ⦃name τ v⦄, old.get name τ = some v → new.get name τ = some v
 
 instance: LT SSAEnv where
   lt := SSAEnv.refines -/
 
+
 -- Interactions manipulating the environment
 
-inductive SSAEnvE: Type → Type where
-  | Get: (α: Type) → SSAVal → SSAEnvE α
+inductive SSAEnvE: Type → Type _ where
+  | Get: (τ: MLIRTy) → [Inhabited τ.eval] → SSAVal → SSAEnvE τ.eval
+  | Set: (τ: MLIRTy) → SSAVal → τ.eval → SSAEnvE Unit
+
+def SSAEnvE.handle: SSAEnvE ~> StateT SSAEnv (Fitree PVoid) :=
+  λ _ e env =>
+    match e with
+    | Get τ name =>
+        match env.get name τ with
+        | some v => return (v, env)
+        | none => return (default, env)
+    | Set τ name v =>
+        return ((), env.set name τ v)
 
 
 -- Tests
 
 private def example_env (l: SSAScope) (s: SSAEnv): SSAEnv :=
-  (⟨"%0", UInt32, 42⟩ :: ⟨"%1", UInt32, 7⟩ :: l) ::
-  (⟨"%3", UInt32, 12⟩ :: ⟨"%res", String, "abc"⟩ :: []) ::
+  (⟨"%0", MLIRTy.int 32, (42:Int)⟩ ::
+   ⟨"%1", MLIRTy.int 32, (7:Int)⟩ ::
+   l) ::
+  (⟨"%3", MLIRTy.int 32, (12:Int)⟩ ::
+   ⟨"%r", MLIRTy.float 32, (-1.7e3:Float)⟩ ::
+   []) ::
   s
 
-example: ∀ l s, SSAEnv.get "%1" (example_env l s) = some ⟨UInt32, 7⟩ :=
-  by simp
-
-
+example: ∀ l s, SSAEnv.get "%1" (MLIRTy.int 32) (example_env l s)
+    = some (7:Int) :=
+  by simp [cast_eq]
